@prefix rdf: <http://www.w3.org/1999/02/22-rdf-syntax-ns#> .
@prefix rdfs: <http://www.w3.org/2000/01/rdf-schema#> .
@prefix owl: <http://www.w3.org/2002/07/owl#> .
@prefix vann: <http://purl.org/vocab/vann/> .
@prefix dcterms: <http://purl.org/dc/terms/> .
@prefix xsd: <http://www.w3.org/2001/XMLSchema#> .
@prefix foaf: <http://xmlns.com/foaf/0.1/> .

@prefix obelisk: <http://w3id.org/obelisk/> .

obelisk: rdf:type owl:Ontology ;
    # Description
    dcterms:title "Obelisk ontology" ;
    dcterms:description """
    The obelisk ontology aims at describing obelisks.
    """ ;
    vann:preferredNamespacePrefix "obelisk" ;
    vann:preferredNamespaceURI <http://w3id.org/obelisk/> ;
    # Ownership
    dcterms:license <https://creativecommons.org/licenses/by/4.0/> ;
    dcterms:creator <https://cleopatra.solidcommunity.net/profile/card#me> ;
    dcterms:contributor <https://jcaesar.solidcommunity.net/profile/card#me> ;
    dcterms:publisher <https://jcaesar.solidcommunity.net/profile/organizations/spqr.ttl#spqr>;
    # Version
    owl:versionIRI <http://w3id.org/obelisk/2019/10/09/ns> ;
    owl:priorVersion <http://w3id.org/obelisk/2019/10/08/ns> ;
    dcterms:isReplacedBy <http://w3id.org/obelisk/2019/10/08/ns> ;
    owl:versionInfo "0.1.0" ;
    dcterms:issued "52BC-01-01" ;
    dcterms:modified "2019-10-09".

obelisk:Obelisk a rdfs:Class ;
    rdfs:label "Obelisk"@en ;
    rdfs:label "Obelisco"@it ;
    rdfs:comment "An obelisk is a four-sided pilar with a pyramid-shaped top."@en ;
    rdfs:comment "Un obelisco è un pilastro a quattro lati con una cima a forma di piramide."@it .

obelisk:Sculptor a rdfs:Class ;
    rdfs:label "Sculptor"@en ;
    rdfs:label "Scultore"@it ;
    rdfs:comment "An artist who sculpts obelisks."@en ;
    rdfs:comment "Un artista che scolpisce obelischi."@it ;
    rdfs:subClassOf foaf:Person .

obelisk:ownedBy a owl:ObjectProperty ;
    rdfs:label "owned by"@en ;
    rdfs:label "posseduto da"@it ;
    rdfs:comment "Relationship between an obelisk and the person who owns it, which is typically the person who ordered it, or to whom it was offered."@en ;
    rdfs:comment "Relazione tra un obelisco e la persona che lo possiede, che in genere è la persona che lo ha ordinato o a chi è stato offerto."@it ;
    rdfs:domain obelisk:Obelisk ;
    rdfs:range foaf:Person .

obelisk:builtBy a owl:ObjectProperty ;
    rdfs:label "built by"@en ;
    rdfs:label "costruito da"@it ;
    rdfs:comment "Relationship between an obelisk and the person who built it."@en ;
    rdfs:comment "Relazione tra un obelisco e la persona che l'ha costruito."@it ;
    rdfs:domain obelisk:Obelisk ;
    rdfs:range obelisk:Sculptor .

obelisk:heigth a owl:DataProperty ;
    rdfs:label "heigth"@en ;
    rdfs:label "altezza"@it ;
    rdfs:comment "The distance from the ground to the highest point of the obelisk, in meters."@en ;
    rdfs:comment "La distanza dal suolo al punto più alto dell'obelisco, in metri."@it ;
    rdfs:domain obelisk:Obelisk ;
    rdfs:range xsd:float.
